Simplify the nonemptiness conditions.

Pythagoras/convex_polygon.lean
@@ -9,7 +9,7 @@ variable [i: incidence_geometry]
 
 def WeakSameside (a b : point) (L : line) : Prop := sameside a b L ∨ online a L ∨ online b L
 
-def list_shift_nat [DecidableEq α] (lst : List α) (_: lst ≠ []) (aL : a ∈ lst) (i : ℕ) : α := by
+def list_shift_nat [DecidableEq α] (lst : List α) (aL : a ∈ lst) (i : ℕ) : α := by
   let n := lst.length
   let j := lst.indexOf a + i
   have : j % n < n := by
@@ -21,35 +21,35 @@ def list_shift_nat [DecidableEq α] (lst : List α) (_: lst ≠ []) (aL : a ∈ 
 /-- ##
   #reduce list_shift ["a", "b", "c", "d"] (by simp) "a" (-1)
  -/
-def list_shift [DecidableEq α] (lst : List α) (ne: lst ≠ []) (aL : a ∈ lst) (i : ℤ) : α := by
+def list_shift [DecidableEq α] (lst : List α) (aL : a ∈ lst) (i : ℤ) : α := by
   cases i with
-  | ofNat j => exact list_shift_nat lst ne aL j
-  | negSucc j => exact list_shift_nat lst ne aL (lst.length - j - 1)
+  | ofNat j => exact list_shift_nat lst aL j
+  | negSucc j => exact list_shift_nat lst aL (lst.length - j - 1)
 
 lemma mem_of_idx (lst : List α) (i : ℕ) {hi: i < List.length lst} : lst[i] ∈ lst := by simp [mem_iff_get]
 
-lemma mem_of_shift [DecidableEq α] (lst : List α) (ne: lst ≠ []) (aL : a ∈ lst) (i : ℤ) : list_shift lst ne aL i ∈ lst := by cases i with | ofNat | negSucc => apply mem_of_idx
+lemma mem_of_shift [DecidableEq α] (lst : List α) (aL : a ∈ lst) (i : ℤ) : list_shift lst aL i ∈ lst := by cases i with | ofNat | negSucc => apply mem_of_idx
 
-lemma same_of_shift_iff [DecidableEq α] (lst : List α) (ne: lst ≠ []) (nodup: lst.Nodup) (aL : a ∈ lst ) (i : ℤ) : list_shift lst ne aL i = a ↔ lst.length % i = 0 := by sorry
+lemma same_of_shift_iff [DecidableEq α] (lst : List α) (nodup: lst.Nodup) (aL : a ∈ lst) (i : ℤ) : list_shift lst aL i = a ↔ lst.length % i = 0 := by sorry
 
-lemma list_shift_1_nat (a b c : point): @list_shift_nat _ a _ [a, b, c] (by simp) (by simp) 1 = b := by dsimp [list_shift_nat]; simp [*]
+lemma list_shift_1_nat (a b c : point): @list_shift_nat _ a _ [a, b, c] (by simp) 1 = b := by dsimp [list_shift_nat]; simp [*]
 
-lemma list_shift_1 (a b c : point): @list_shift _ a _ [a, b, c] (by simp) (by simp) 1 = b := by conv => rhs; rw [← list_shift_1_nat a b c]
+lemma list_shift_1 (a b c : point): @list_shift _ a _ [a, b, c] (by simp) 1 = b := by conv => rhs; rw [← list_shift_1_nat a b c]
 
-def convex (V: List point) (ne: V ≠ []) : Prop :=
+def convex (V: List point) : Prop :=
   ∀ a b c : point, ∀ L : line,
-  (aV: a ∈ V) -> (b ∈ V) → (c ∈ V) → (online a L) → (online (list_shift V ne aV 1) L) → WeakSameside b c L
+  (aV: a ∈ V) -> (b ∈ V) → (c ∈ V) → (online a L) → (online (list_shift V aV 1) L) → WeakSameside b c L
 
-lemma convex_of_sublist (C: convex V nV) (sub: W <+ V) (nW: W ≠ []) : convex W nW := by sorry
+lemma convex_of_sublist (C: convex V) (sub: W <+ V) (nW: W ≠ []) : convex W := by sorry
 
 structure ConvexPolygon where
   vertices : List point
-  nonempty: vertices ≠ [] := by simpa
   nodup : Nodup vertices
-  convex: convex vertices nonempty
+  convex: convex vertices
+  nondeg: vertices ≠ [] := by simp
 
 lemma triangle_is_convex (T: triangle a b c) : ConvexPolygon := by
-  refine ConvexPolygon.mk [a,b,c] (by simp) ?_ ?_
+  refine ConvexPolygon.mk [a,b,c] ?_ ?_
   perm [ne_12_of_tri T, ne_13_of_tri T, ne_23_of_tri T]; simp; tauto
   dsimp [convex, WeakSameside]
   intro x y z L xP yP zP xL wL
@@ -58,8 +58,8 @@ lemma triangle_is_convex (T: triangle a b c) : ConvexPolygon := by
     have : n = (0 : Fin 3) := by sorry -- WLOG
     simp [*] at hn
     exact hn.symm
-  let w := list_shift [a, b, c] (by simp) xP 1
-  have wP : w ∈ [a, b, c] := mem_of_shift [a,b,c] (by simp) xP 1
+  let w := list_shift [a, b, c] xP 1
+  have wP : w ∈ [a, b, c] := mem_of_shift [a,b,c] xP 1
   have wb : w = b := by simp [xa]; exact list_shift_1 a b c
   simp [*, list_shift_1] at wL; rw [← wb] at wL
   have aL : online a L := by rwa [← xa]
@@ -97,7 +97,7 @@ def ConvexPolygon_remove_vertex [DecidableEq point] (P : ConvexPolygon) (a b : p
     apply (@eq_nil_iff_forall_not_mem point (P.vertices.diff [a])).mp empty b
     convert mem_diff_single_of_ne bP ab
   have convex := convex_of_sublist P.convex (diff_sublist P.vertices [a]) ne
-  exact ConvexPolygon.mk V ne (Nodup.diff P.nodup) convex
+  exact ConvexPolygon.mk V (Nodup.diff P.nodup) convex ne
 
 #exit
 def Fin.neZero_of (i : Fin n) : NeZero n := ⟨Nat.pos_iff_ne_zero.mp (Fin.pos i)⟩
